# A simple process

- Since ```8.8 + sqrt(square(x)  + square(y)) = sqrt(square(10.2 - x) + square(y))```

- Square the expression -> 

```square(8.8) + square(x) + square(y) + 2 * 8.8 * sqrt(square(x) + square(y)) = square(10.2 - x) + square(y)```

- Conclude that 

```2 * 8.8 * sqrt(square(x) + square(y)) = square(10.2) - square(8.8) - 2 * 10.2 * x```

- Finally we got       

```square(x) + square(y) = square( (13.3 - 10.2 * x) / 8.8 )```

That is ```y = +/- sqrt( square( (13.3 -  10.2 * x) / 8.8 ) - square( x * x) )```  

